merge from list

heap.c
@@ -13,27 +13,28 @@ void swap(int *a, int *b) {
 }
 
 void up(int *a, int pos) {
-  /*@ With Hl Maxsize size0 pos0     
+  /*@ With Hl Maxsize size0 pos0 a0 
       Require 
+        all_int(Hl) && 2 <= Maxsize && Maxsize <= INT_MAX &&
         1 <= pos0 && pos0 <= size0 &&
-        1 <= size0 && size0 <= Maxsize &&   
-        pos == Vint (IntRepr (pos0)) &&  
-        MaxHeap(Hl, pos0 - 1) && MaxHeap_p(Hl, pos0, size0) &&
-        store_int_array(a, Hl, Maxsize)
+        1 <= size0 && size0 + 1 <= Maxsize && a == a0 &&
+        pos == Vint (IntRepr (pos0)) && 
+        store_int_array(a0, Hl, Maxsize)
       Ensure 
         exists Hl_final pos1,
-          pos == Vint (IntRepr (pos1)) && 
           up(Hl, size0, pos0, pos1, Hl_final) && 
-          MaxHeap(Hl_final, size0) && 
-          store_int_array(a, Hl_final, Maxsize)
+          store_int_array(a0, Hl_final, Maxsize)
   */
 
   /*@ Inv
         exists Hl0 pos1, 
-          pos == Vint (IntRepr (pos1)) &&  
-          up(Hl, size0, pos0, pos1, Hl0) &&
-          MaxHeap(Hl0, pos1 - 1) && MaxHeap_p(Hl0, pos1, size0) &&  
-          store_int_array(a, Hl0, Maxsize)
+          all_int(Hl) && 2 <= Maxsize && Maxsize <= INT_MAX &&
+          1 <= pos0 && pos0 <= size0 &&
+          1 <= size0 && size0 + 1 <= Maxsize &&   
+          1 <= pos1 && pos1 <= size0 && a == a0 &&
+          pos == Vint (IntRepr (pos1)) && 
+          up_inv(Hl, size0, pos0, pos1, Hl0) &&
+          store_int_array(a0, Hl0, Maxsize)
   */
   while (pos > 1) {
     if (a[pos] <= a[pos >> 1]) {
@@ -45,32 +46,32 @@ void up(int *a, int pos) {
 }
 
 void down(int *a, int size, int pos) {
-  /*@ With Hl Maxsize size0 pos0    
+  /*@ With Hl Maxsize size0 pos0 a0
       Require 
+        all_int(Hl) && 2 <= Maxsize && Maxsize <= INT_MAX &&
         1 <= pos0 && pos0 <= size0 &&
-        1 <= size0 && size0 <= Maxsize && 
+        1 <= size0 && size0 + 1 <= Maxsize && a == a0 &&
         pos == Vint (IntRepr (pos0)) && 
         size == Vint (IntRepr (size0)) &&  
-        MaxHeap(Hl, pos0) && MaxHeap_p(Hl, pos0 + 1, size0) &&
-        store_int_array(a, Hl, Maxsize)
+        store_int_array(a0, Hl, Maxsize)
       Ensure 
         exists Hl_final pos1,
           pos1 <= size0 && 
-          pos == Vint (IntRepr (pos1)) &&
-          size == Vint (IntRepr (size0)) &&  
           down(Hl, size0, pos0, pos1, Hl_final) && 
-          MaxHeap(Hl_final, size0) && 
-          store_int_array(a, Hl_final, Maxsize)
+          store_int_array(a0, Hl_final, Maxsize)
   */
 
   /*@ Inv
         exists Hl0 pos1, 
+          all_int(Hl) && 2 <= Maxsize && Maxsize <= INT_MAX &&
+          1 <= pos0 && pos0 <= size0 &&
+          1 <= size0 && size0 + 1 <= Maxsize &&   
+          1 <= pos1 && pos1 <= size0 && a == a0 &&
           pos1 <= size0 && 
-          pos == Vint (IntRepr (pos1)) && 
-          size == Vint (IntRepr (size0)) && 
-          down(Hl, size0, pos0, pos1, Hl0) &&
-          MaxHeap(Hl0, pos1) && MaxHeap_p(Hl0, pos1 + 1, size0) &&  
-          store_int_array(a, Hl0, Maxsize)
+          pos == Vint (IntRepr (pos1)) &&
+          size == Vint (IntRepr (size0)) &&  
+          down_inv(Hl, size0, pos0, pos1, Hl0) &&
+          store_int_array(a0, Hl0, Maxsize)
   */
   while (pos << 1 <= size) {
     int t;
@@ -92,41 +93,37 @@ void down(int *a, int size, int pos) {
 }
 
 void push(int *a, int *size, int val) {
-  /*@ With Hl Maxsize size0 val0    
+  /*@ With Hl Maxsize size0 size_p val0 a0
       Require 
-        0 <= size0 && size0 < Maxsize &&
+        all_int(Hl) && INT_MIN <= val0 && val0 <= INT_MAX &&
+        1 <= Maxsize && Maxsize <= INT_MAX &&
+        0 <= size0 && size0 + 1 + 1 <= Maxsize && a0 == a && 
         val == Vint (IntRepr (val0)) && 
-        size == Vint (IntRepr (size0)) &&  
-        MaxHeap(Hl, size0) &&
-        store_int_array(a, Hl, Maxsize)
+        size == size_p && 
+        store_int_array(a0, Hl, Maxsize) * store_int(size_p, size0)
       Ensure 
         exists Hl_final,
-          val == Vint (IntRepr (val0)) && 
-          size == Vint (IntRepr (size0 + 1)) && 
           push(Hl, size0, val0, Hl_final) && 
-          MaxHeap(Hl_final, size0 + 1) && 
-          store_int_array(a, Hl_final, Maxsize)
+          store_int_array(a0, Hl_final, Maxsize) * store_int(size_p, size0 + 1)
   */
-  ++(*size);
+  (*size) = (*size) + 1;
   a[*size] = val;
   up(a, *size);
 }
 
 int pop(int *a, int *size) {
-  /*@ With Hl Maxsize size0    
+  /*@ With Hl Maxsize size0 size_p a0
       Require  
-        0 <= size0 && size0 <= Maxsize &&
-        size == Vint (IntRepr (size0)) &&  
-        MaxHeap(Hl, size0) &&
-        store_int_array(a, Hl, Maxsize)
+        all_int(Hl) && 1 <= Maxsize && Maxsize <= INT_MAX &&
+        0 <= size0 && size0 + 1 <= Maxsize && a == a0 &&
+        size == size_p && 
+        store_int_array(a0, Hl, Maxsize) * store_int(size_p, size0)
       Ensure 
         exists Hl_final size1,
           __return == Vint (IntRepr (pop_result(Hl, size0))) && 
           size1 == pop_length(Hl, size0) && 
-          size == Vint (IntRepr (size1)) && 
           pop(Hl, size0, Hl_final) && 
-          MaxHeap(Hl_final, size1) && 
-          store_int_array(a, Hl_final, Maxsize)
+          store_int_array(a0, Hl_final, Maxsize) * store_int(size_p, size1)
   */
   if (*size == 0)
   {
@@ -139,9 +136,10 @@ int pop(int *a, int *size) {
 }
 
 int top(int *a) {
-  /*@ With Hl Maxsize 
-      Require Maxsize >= 2 && store_int_array(a, Hl, Maxsize)
-      Ensure __return == Vint (IntRepr (Znth(1, Hl))) && store_int_array(a, Hl, Maxsize)
+  /*@ With Hl Maxsize a0
+      Require a == a0 && 2 <= Maxsize && Maxsize <= INT_MAX && store_int_array(a0, Hl, Maxsize)
+      
+      Ensure __return == Vint (IntRepr (Znth(1, Hl))) && store_int_array(a0, Hl, Maxsize)
   */
   return a[1];
 }
