heap/down/verif.v
@@ -1,22 +1,22 @@
 Require Import utils.VSTALib.
 
-Require Import cprogs.heap.program.
-Require Import cprogs.heap.definitions.
-Require Import cprogs.heap.annotation.
-Require cprogs.heap.down.path0_verif.
-Require cprogs.heap.down.path1_verif.
-Require cprogs.heap.down.path2_verif.
-Require cprogs.heap.down.path3_verif.
-Require cprogs.heap.down.path4_verif.
-Require cprogs.heap.down.path5_verif.
-Require cprogs.heap.down.path6_verif.
-Require cprogs.heap.down.path7_verif.
-Require cprogs.heap.down.path8_verif.
-Require cprogs.heap.down.path9_verif.
-Require cprogs.heap.down.path10_verif.
-Require cprogs.heap.down.path11_verif.
-Require cprogs.heap.down.path12_verif.
-Require cprogs.heap.down.path13_verif.
+Require Import heap.program.
+Require Import heap.definitions.
+Require Import heap.annotation.
+Require heap.down.path0_verif.
+Require heap.down.path1_verif.
+Require heap.down.path2_verif.
+Require heap.down.path3_verif.
+Require heap.down.path4_verif.
+Require heap.down.path5_verif.
+Require heap.down.path6_verif.
+Require heap.down.path7_verif.
+Require heap.down.path8_verif.
+Require heap.down.path9_verif.
+Require heap.down.path10_verif.
+Require heap.down.path11_verif.
+Require heap.down.path12_verif.
+Require heap.down.path13_verif.
 
 Theorem f_down_functionally_correct :
   semax_body Vprog Gprog f_down down_spec.
