heap/pop/verif.v
@@ -1,10 +1,10 @@
 Require Import utils.VSTALib.
 
-Require Import cprogs.heap.program.
-Require Import cprogs.heap.definitions.
-Require Import cprogs.heap.annotation.
-Require cprogs.heap.pop.ret_path0_verif.
-Require cprogs.heap.pop.ret_path1_verif.
+Require Import heap.program.
+Require Import heap.definitions.
+Require Import heap.annotation.
+Require heap.pop.ret_path0_verif.
+Require heap.pop.ret_path1_verif.
 
 Theorem f_pop_functionally_correct :
   semax_body Vprog Gprog f_pop pop_spec.
