heap/push/path0_verif.v
@@ -1,17 +1,21 @@
 Require Import utils.VSTALib.
 
-Require Import cprogs.heap.program.
-Require Import cprogs.heap.definitions.
-Require Import cprogs.heap.annotation.
-Require cprogs.heap.push.path0.
+Require Import heap.program.
+Require Import heap.definitions.
+Require Import heap.annotation.
+Require heap.push.path0.
 
 Module SH_Proof <: STRAIGHTLINE_HOARE_TRIPLE_PROOF.
 
-Include cprogs.heap.push.path0.
+Include heap.push.path0.
 
 Theorem proof: functional_correctness_statement.
 Proof.
   cbv delta [functional_correctness_statement].
+  intros; Intros; subst.
+  forward. forward. forward. forward. forward.
+  forward_call ((size0+1), (size0+1), a', Maxsize, Hl ++ [val0], a', (Vint (IntRepr (size0+1)))).
+  
 Admitted.
 
 End SH_Proof.
