heap/swap/path0_verif.v
@@ -1,17 +1,20 @@
 Require Import utils.VSTALib.
 
-Require Import cprogs.heap.program.
-Require Import cprogs.heap.definitions.
-Require Import cprogs.heap.annotation.
-Require cprogs.heap.swap.path0.
+Require Import heap.program.
+Require Import heap.definitions.
+Require Import heap.annotation.
+Require heap.swap.path0.
 
 Module SH_Proof <: STRAIGHTLINE_HOARE_TRIPLE_PROOF.
 
-Include cprogs.heap.swap.path0.
+Include heap.swap.path0.
 
 Theorem proof: functional_correctness_statement.
 Proof.
   cbv delta [functional_correctness_statement].
-Admitted.
+  intros; Intros; subst.
+  forward. forward. forward. forward.
+  entailer!.
+Qed.
 
 End SH_Proof.
