heap/top/ret_path0_verif.v
@@ -1,27 +1,23 @@
 Require Import utils.VSTALib.
 
-Require Import cprogs.heap.program.
-Require Import cprogs.heap.definitions.
-Require Import cprogs.heap.annotation.
-Require cprogs.heap.top.ret_path0.
+Require Import heap.program.
+Require Import heap.definitions.
+Require Import heap.annotation.
+Require heap.top.ret_path0.
 
 Module SH_Proof <: STRAIGHTLINE_HOARE_TRIPLE_PROOF.
 
-Include cprogs.heap.top.ret_path0.
+Include heap.top.ret_path0.
 
 Theorem proof: functional_correctness_statement.
 Proof.
   cbv delta [functional_correctness_statement].
-  intros.
+  intros; Intros; subst.
+  sep_apply list_length; [lia|].
   Intros.
-  (* forward. *)
-  sep_apply list_length; [lia |].
-  Intros.
-  forward.
-  unfold POSTCONDITION.
-  unfold abbreviate.
-  
-  forward.
-Admitted.
+  forward. forward.
+  Exists  (Vint (IntRepr (Znth 1 Hl))).
+  entailer!.
+Qed.
 
 End SH_Proof.
