heap/top/verif.v
@@ -1,9 +1,9 @@
 Require Import utils.VSTALib.
 
-Require Import cprogs.heap.program.
-Require Import cprogs.heap.definitions.
-Require Import cprogs.heap.annotation.
-Require cprogs.heap.top.ret_path0_verif.
+Require Import heap.program.
+Require Import heap.definitions.
+Require Import heap.annotation.
+Require heap.top.ret_path0_verif.
 
 Theorem f_top_functionally_correct :
   semax_body Vprog Gprog f_top top_spec.
