heap/up/path0.v
@@ -10,21 +10,21 @@ Require Import Csplit.strongSoundness.
 Require Import Csplit.AClightFunc.
 Local Open Scope Z_scope.
 Import AClightNotations.
-Require Import cprogs.heap.program.
-Require Import cprogs.heap.definitions.
-Require Import cprogs.heap.annotation.
+Require Import heap.program.
+Require Import heap.definitions.
+Require Import heap.annotation.
 Import compcert.cfrontend.Clight.
 
 Definition functional_correctness_statement: Prop :=
-  forall (Espec: OracleKind) Hl Maxsize size0 pos0 a' pos',
+  forall (Espec: OracleKind) Hl Maxsize size0 pos0 a0 a' pos',
   let Delta_specs := Delta_specs_up in
   let Delta := Delta_up Delta_specs in
-  semax Delta (PROP ((MaxHeap_p Hl pos0 size0); (MaxHeap Hl (Z.sub pos0 1)); (pos' = (Vint (IntRepr pos0))); (Z.le size0 Maxsize); (Z.le 1 size0); (Z.le pos0 size0); (Z.le 1 pos0))
+  semax Delta (PROP ((pos' = (Vint (IntRepr pos0))); (a' = a0); (Z.le (Z.add size0 1) Maxsize); (Z.le 1 size0); (Z.le pos0 size0); (Z.le 1 pos0); (Z.le Maxsize (Int.max_signed )); (Z.le 2 Maxsize); (all_int Hl))
   LOCAL (temp _a a'; temp _pos pos')
-  SEP ((store_int_array a' Hl Maxsize)))
+  SEP ((store_int_array a0 Hl Maxsize)))
   Sskip
   (normal_split_assert
   (EX Hl0 pos1 a pos,
-    (PROP ((MaxHeap_p Hl0 pos1 size0); (MaxHeap Hl0 (Z.sub pos1 1)); (up Hl size0 pos0 pos1 Hl0); (pos = (Vint (IntRepr pos1))))
+    (PROP ((up_inv Hl size0 pos0 pos1 Hl0); (pos = (Vint (IntRepr pos1))); (a = a0); (Z.le pos1 size0); (Z.le 1 pos1); (Z.le (Z.add size0 1) Maxsize); (Z.le 1 size0); (Z.le pos0 size0); (Z.le 1 pos0); (Z.le Maxsize (Int.max_signed )); (Z.le 2 Maxsize); (all_int Hl))
     LOCAL (temp _a a; temp _pos pos)
-    SEP ((store_int_array a Hl0 Maxsize))))%assert).
+    SEP ((store_int_array a0 Hl0 Maxsize))))%assert).
