heap/up/verif.v
@@ -1,12 +1,12 @@
 Require Import utils.VSTALib.
 
-Require Import cprogs.heap.program.
-Require Import cprogs.heap.definitions.
-Require Import cprogs.heap.annotation.
-Require cprogs.heap.up.path0_verif.
-Require cprogs.heap.up.path1_verif.
-Require cprogs.heap.up.path2_verif.
-Require cprogs.heap.up.path3_verif.
+Require Import heap.program.
+Require Import heap.definitions.
+Require Import heap.annotation.
+Require heap.up.path0_verif.
+Require heap.up.path1_verif.
+Require heap.up.path2_verif.
+Require heap.up.path3_verif.
 
 Theorem f_up_functionally_correct :
   semax_body Vprog Gprog f_up up_spec.
